chore(KSA-Model): more Mutation Operation changes (#955)
Explicitly:
- Change InitializeMutationFlag from a union to an enum for ToString reasons
- Model `DoNotVersion` flag for Initialize Mutation
- Refactor Describe Mutation output to detail Input so resume can be done
- Refactor System Key to be optional, detailing that TrustStorage is the default
- More errors
- Smithy changes from PR feedback on #854
- Correction of spelling mistakes
- Mutation Token's UUID is required

Why change the flag to an enum?

Dafny/Smithy-Dafny's support for Union's results in structures that do not print well.
The intention of the  `InitializeMutationFlag` is to inform customers
about the result of their request.

Such information may,
possibly even should,
be logged.

Initialize Mutation and Apply Mutation MUST
ensure that the UUID of the Index and Commitment agree.
Apply MUST ensure that the UUID of the Commitment and Token agree.
The Mutation Token's UUID is REQUIRED.
It is how we track a mutation,
much like how CFN tracks a change set.

Fixed bug where UUID is a reserved word in DDB.

Refactored some of the error messages.
Utilize Java Example to demonstrate resume and restart.
Finally, addressed some of the feedback on PR #854.

feat(Mutations): Idempotent Resume (#854)

Refactor Storage:
- Rename Mutation Lock to Mutation Commitment
- Introduce Mutation Index to describe what items of a Branch Key have been mutated
- Add Input field to Mutation Commitment
- Add Ciphertext field to Mutation Commitment
- When Mutating an item, always write with an optimistic lock
- Allow Initialize Mutation to over write a Version, instead of only creating a version
- When Overwriting a Mutation Index, ensure it has not changed
- Whenever writing for Mutation, ensure the Mutation Commitment's ENC is as expected (along with original and terminal)

Refactor Storage to contain operations that:
1. Allow for Atomic Mutations (maybe cut later)
2. Allow for Deleting a Mutation
3. Allow for Creating a Mutation Index

Refactor KeyStoreAdmin:
- Support a System Key for Mutations
- Stub out the System Key
- Logic for handling Mutation Index

Refactor Initialize Mutation:
- If Commitment & Index already exist and match Input, write nothing and return token
- If Commitment already exists and matches input, write index, and return token
- If Commitment already exists and does not match input, fail
- If no commitment, Initialize Mutation

Refactor Apply Mutation:
- Write an update Page Index.

fix: Dafny intendation formatting

chore: fix Java test examples

chore: more fomratting for CI

feat(Mutations): Native test for Loose access in-flight

feat(Mutations): Example In Flight Mutation Scanner

feat(Mutations-TODO): Some Terminal KMS Exceptions (#795)

If the KMS Call, for mutating the Beacon, fails,
it MAY indicate the MPL Consumer does not have access to the
terminal KMS Key.

If the KMS call for verifying a terminal version fails,
it MAY indicate the MPL Consumer does not have access to the
terminal KMS Key.

Also fix some Dafny tests failing verification.

feat(KS+): More modeled errors (#754)

* refactor(Storage): Use TransactGet instead of BatchGet for GetInitMut (#753)

This resolves feedback from both @seebees  and @josecorella
on Mutations branch.

* chore(Mutations): address #754\#discussion_r1775676091

https://github.com/aws/aws-cryptographic-material-providers-library/pull/754#discussion_r1775673683

* chore(Mutations): Address feedback from #750

See https://github.com/aws/aws-cryptographic-material-providers-library/pull/750

* chore(Mutations): address feedback on #742

See https://github.com/aws/aws-cryptographic-material-providers-library/pull/742

refactor(Storage): Use TransactGet instead of BatchGet for GetInitMut (#753)

This resolves feedback from both @seebees  and @josecorella
on Mutations branch.

Verification failure is due to (just like in #751 ):
1. Key Store Admin's Index.dfy not proving Fresh, which has been a long standing issue with the Admin
2. In `AwsCryptographyKeyStore/test/Storage/TestGetItemsForInitializeMutation.dfy`, the test assumes `type` is in the Encryption Context. It is, but Structure.dfy does not prove that, so it must be proven else where.

A .NET MPL job failed due to .NET 48 Sig V4 Auth bug.

test(Mutations): additional testing for Mutations

feat(Mutations): more clean up

feat(Mutations): log statements for ApplyMutation

fix(Storage): typo

fix(Storage): ensure KmsArn is valid

chore(Mutations): respond to comments on PR #720

test(GHW): Run Java Examples for PR CI (#749)

chore(Java): Examples for Mutations (#742)

chore(Mutations): comment out non-GA Mutations (#750)

Crypto Tools, at this time, intends to release Branch Key Mutations
without some operations useful for recovering a dropped Mutation Token
or dealing with the disagreement of a Mutation Token and a Mutation Lock.

Additionally,
we intend to release the Key Store Admin with only support for
one Key Management Strategy.

All checks are green except for Verification.
Verification is failing for the Key Store Admin's Index.dfy.

Verification for the Key Store Admin's Index.dfy
has been failing for a long time.

feat: Mutations BETA (#720)

Beta build of Mutations with several substantial gaps

AwsCryptographicMaterialProviders/runtimes/go/ImplementationFromDafny-go/awscryptographykeystoresmithygenerated/to_native.go
@@ -102,15 +102,15 @@ func VersionKeyOutput_FromDafny(dafnyOutput AwsCryptographyKeyStoreTypes.Version
 
 }
 
-func GetEncryptedActiveBranchKeyInput_FromDafny(dafnyInput AwsCryptographyKeyStoreTypes.GetEncryptedActiveBranchKeyInput) awscryptographykeystoresmithygeneratedtypes.GetEncryptedActiveBranchKeyInput {
+func DeleteMutationInput_FromDafny(dafnyInput AwsCryptographyKeyStoreTypes.DeleteMutationInput) awscryptographykeystoresmithygeneratedtypes.DeleteMutationInput {
 
-	return awscryptographykeystoresmithygeneratedtypes.GetEncryptedActiveBranchKeyInput{Identifier: aws_cryptography_keyStore_GetEncryptedActiveBranchKeyInput_Identifier_FromDafny(dafnyInput.Dtor_Identifier())}
+	return awscryptographykeystoresmithygeneratedtypes.DeleteMutationInput{MutationCommitment: aws_cryptography_keyStore_DeleteMutationInput_MutationCommitment_FromDafny(dafnyInput.Dtor_MutationCommitment())}
 
 }
 
-func GetEncryptedActiveBranchKeyOutput_FromDafny(dafnyOutput AwsCryptographyKeyStoreTypes.GetEncryptedActiveBranchKeyOutput) awscryptographykeystoresmithygeneratedtypes.GetEncryptedActiveBranchKeyOutput {
+func DeleteMutationOutput_FromDafny(dafnyOutput AwsCryptographyKeyStoreTypes.DeleteMutationOutput) awscryptographykeystoresmithygeneratedtypes.DeleteMutationOutput {
 
-	return awscryptographykeystoresmithygeneratedtypes.GetEncryptedActiveBranchKeyOutput{Item: aws_cryptography_keyStore_GetEncryptedActiveBranchKeyOutput_Item_FromDafny(dafnyOutput.Dtor_Item())}
+	return awscryptographykeystoresmithygeneratedtypes.DeleteMutationOutput{}
 
 }
 
@@ -121,6 +121,18 @@ func KeyStorageInterface_FromDafny(dafnyResource AwsCryptographyKeyStoreTypes.IK
 	}
 
 	return &KeyStorageInterface{dafnyResource}
+}
+
+func GetEncryptedActiveBranchKeyInput_FromDafny(dafnyInput AwsCryptographyKeyStoreTypes.GetEncryptedActiveBranchKeyInput) awscryptographykeystoresmithygeneratedtypes.GetEncryptedActiveBranchKeyInput {
+
+	return awscryptographykeystoresmithygeneratedtypes.GetEncryptedActiveBranchKeyInput{Identifier: aws_cryptography_keyStore_GetEncryptedActiveBranchKeyInput_Identifier_FromDafny(dafnyInput.Dtor_Identifier())}
+
+}
+
+func GetEncryptedActiveBranchKeyOutput_FromDafny(dafnyOutput AwsCryptographyKeyStoreTypes.GetEncryptedActiveBranchKeyOutput) awscryptographykeystoresmithygeneratedtypes.GetEncryptedActiveBranchKeyOutput {
+
+	return awscryptographykeystoresmithygeneratedtypes.GetEncryptedActiveBranchKeyOutput{Item: aws_cryptography_keyStore_GetEncryptedActiveBranchKeyOutput_Item_FromDafny(dafnyOutput.Dtor_Item())}
+
 }
 
 func GetEncryptedBeaconKeyInput_FromDafny(dafnyInput AwsCryptographyKeyStoreTypes.GetEncryptedBeaconKeyInput) awscryptographykeystoresmithygeneratedtypes.GetEncryptedBeaconKeyInput {
@@ -149,6 +161,22 @@ func GetEncryptedBranchKeyVersionOutput_FromDafny(dafnyOutput AwsCryptographyKey
 
 }
 
+func GetItemsForInitializeMutationInput_FromDafny(dafnyInput AwsCryptographyKeyStoreTypes.GetItemsForInitializeMutationInput) awscryptographykeystoresmithygeneratedtypes.GetItemsForInitializeMutationInput {
+
+	return awscryptographykeystoresmithygeneratedtypes.GetItemsForInitializeMutationInput{Identifier: aws_cryptography_keyStore_GetItemsForInitializeMutationInput_Identifier_FromDafny(dafnyInput.Dtor_Identifier())}
+
+}
+
+func GetItemsForInitializeMutationOutput_FromDafny(dafnyOutput AwsCryptographyKeyStoreTypes.GetItemsForInitializeMutationOutput) awscryptographykeystoresmithygeneratedtypes.GetItemsForInitializeMutationOutput {
+
+	return awscryptographykeystoresmithygeneratedtypes.GetItemsForInitializeMutationOutput{ActiveItem: aws_cryptography_keyStore_GetItemsForInitializeMutationOutput_ActiveItem_FromDafny(dafnyOutput.Dtor_ActiveItem()),
+		BeaconItem:         aws_cryptography_keyStore_GetItemsForInitializeMutationOutput_BeaconItem_FromDafny(dafnyOutput.Dtor_BeaconItem()),
+		MutationCommitment: aws_cryptography_keyStore_GetItemsForInitializeMutationOutput_MutationCommitment_FromDafny(dafnyOutput.Dtor_MutationCommitment().UnwrapOr(nil)),
+		MutationIndex:      aws_cryptography_keyStore_GetItemsForInitializeMutationOutput_MutationIndex_FromDafny(dafnyOutput.Dtor_MutationIndex().UnwrapOr(nil)),
+	}
+
+}
+
 func GetKeyStorageInfoInput_FromDafny(dafnyInput AwsCryptographyKeyStoreTypes.GetKeyStorageInfoInput) awscryptographykeystoresmithygeneratedtypes.GetKeyStorageInfoInput {
 
 	return awscryptographykeystoresmithygeneratedtypes.GetKeyStorageInfoInput{}
@@ -160,6 +188,100 @@ func GetKeyStorageInfoOutput_FromDafny(dafnyOutput AwsCryptographyKeyStoreTypes.
 	return awscryptographykeystoresmithygeneratedtypes.GetKeyStorageInfoOutput{Name: aws_cryptography_keyStore_GetKeyStorageInfoOutput_Name_FromDafny(dafnyOutput.Dtor_Name()),
 		LogicalName: aws_cryptography_keyStore_GetKeyStorageInfoOutput_LogicalName_FromDafny(dafnyOutput.Dtor_LogicalName()),
 	}
+
+}
+
+func GetMutationInput_FromDafny(dafnyInput AwsCryptographyKeyStoreTypes.GetMutationInput) awscryptographykeystoresmithygeneratedtypes.GetMutationInput {
+
+	return awscryptographykeystoresmithygeneratedtypes.GetMutationInput{Identifier: aws_cryptography_keyStore_GetMutationInput_Identifier_FromDafny(dafnyInput.Dtor_Identifier())}
+
+}
+
+func GetMutationOutput_FromDafny(dafnyOutput AwsCryptographyKeyStoreTypes.GetMutationOutput) awscryptographykeystoresmithygeneratedtypes.GetMutationOutput {
+
+	return awscryptographykeystoresmithygeneratedtypes.GetMutationOutput{MutationCommitment: aws_cryptography_keyStore_GetMutationOutput_MutationCommitment_FromDafny(dafnyOutput.Dtor_MutationCommitment().UnwrapOr(nil)),
+		MutationIndex: aws_cryptography_keyStore_GetMutationOutput_MutationIndex_FromDafny(dafnyOutput.Dtor_MutationIndex().UnwrapOr(nil)),
+	}
+
+}
+
+func QueryForVersionsInput_FromDafny(dafnyInput AwsCryptographyKeyStoreTypes.QueryForVersionsInput) awscryptographykeystoresmithygeneratedtypes.QueryForVersionsInput {
+
+	return awscryptographykeystoresmithygeneratedtypes.QueryForVersionsInput{ExclusiveStartKey: aws_cryptography_keyStore_QueryForVersionsInput_ExclusiveStartKey_FromDafny(dafnyInput.Dtor_ExclusiveStartKey().UnwrapOr(nil)),
+		Identifier: aws_cryptography_keyStore_QueryForVersionsInput_Identifier_FromDafny(dafnyInput.Dtor_Identifier()),
+		PageSize:   aws_cryptography_keyStore_QueryForVersionsInput_PageSize_FromDafny(dafnyInput.Dtor_PageSize()),
+	}
+
+}
+
+func QueryForVersionsOutput_FromDafny(dafnyOutput AwsCryptographyKeyStoreTypes.QueryForVersionsOutput) awscryptographykeystoresmithygeneratedtypes.QueryForVersionsOutput {
+
+	return awscryptographykeystoresmithygeneratedtypes.QueryForVersionsOutput{ExclusiveStartKey: aws_cryptography_keyStore_QueryForVersionsOutput_ExclusiveStartKey_FromDafny(dafnyOutput.Dtor_ExclusiveStartKey()),
+		Items: aws_cryptography_keyStore_QueryForVersionsOutput_Items_FromDafny(dafnyOutput.Dtor_Items()),
+	}
+
+}
+
+func WriteAtomicMutationInput_FromDafny(dafnyInput AwsCryptographyKeyStoreTypes.WriteAtomicMutationInput) awscryptographykeystoresmithygeneratedtypes.WriteAtomicMutationInput {
+
+	return awscryptographykeystoresmithygeneratedtypes.WriteAtomicMutationInput{Active: aws_cryptography_keyStore_WriteAtomicMutationInput_Active_FromDafny(dafnyInput.Dtor_Active()),
+		Version: aws_cryptography_keyStore_WriteAtomicMutationInput_Version_FromDafny(dafnyInput.Dtor_Version()),
+		Beacon:  aws_cryptography_keyStore_WriteAtomicMutationInput_Beacon_FromDafny(dafnyInput.Dtor_Beacon()),
+		Items:   aws_cryptography_keyStore_WriteAtomicMutationInput_Items_FromDafny(dafnyInput.Dtor_Items()),
+	}
+
+}
+
+func WriteAtomicMutationOutput_FromDafny(dafnyOutput AwsCryptographyKeyStoreTypes.WriteAtomicMutationOutput) awscryptographykeystoresmithygeneratedtypes.WriteAtomicMutationOutput {
+
+	return awscryptographykeystoresmithygeneratedtypes.WriteAtomicMutationOutput{}
+
+}
+
+func WriteInitializeMutationInput_FromDafny(dafnyInput AwsCryptographyKeyStoreTypes.WriteInitializeMutationInput) awscryptographykeystoresmithygeneratedtypes.WriteInitializeMutationInput {
+
+	return awscryptographykeystoresmithygeneratedtypes.WriteInitializeMutationInput{Active: aws_cryptography_keyStore_WriteInitializeMutationInput_Active_FromDafny(dafnyInput.Dtor_Active()),
+		Version:            aws_cryptography_keyStore_WriteInitializeMutationInput_Version_FromDafny(dafnyInput.Dtor_Version()),
+		Beacon:             aws_cryptography_keyStore_WriteInitializeMutationInput_Beacon_FromDafny(dafnyInput.Dtor_Beacon()),
+		MutationCommitment: aws_cryptography_keyStore_WriteInitializeMutationInput_MutationCommitment_FromDafny(dafnyInput.Dtor_MutationCommitment()),
+		MutationIndex:      aws_cryptography_keyStore_WriteInitializeMutationInput_MutationIndex_FromDafny(dafnyInput.Dtor_MutationIndex()),
+	}
+
+}
+
+func WriteInitializeMutationOutput_FromDafny(dafnyOutput AwsCryptographyKeyStoreTypes.WriteInitializeMutationOutput) awscryptographykeystoresmithygeneratedtypes.WriteInitializeMutationOutput {
+
+	return awscryptographykeystoresmithygeneratedtypes.WriteInitializeMutationOutput{}
+
+}
+
+func WriteMutatedVersionsInput_FromDafny(dafnyInput AwsCryptographyKeyStoreTypes.WriteMutatedVersionsInput) awscryptographykeystoresmithygeneratedtypes.WriteMutatedVersionsInput {
+
+	return awscryptographykeystoresmithygeneratedtypes.WriteMutatedVersionsInput{Items: aws_cryptography_keyStore_WriteMutatedVersionsInput_Items_FromDafny(dafnyInput.Dtor_Items()),
+		MutationCommitment: aws_cryptography_keyStore_WriteMutatedVersionsInput_MutationCommitment_FromDafny(dafnyInput.Dtor_MutationCommitment()),
+		MutationIndex:      aws_cryptography_keyStore_WriteMutatedVersionsInput_MutationIndex_FromDafny(dafnyInput.Dtor_MutationIndex()),
+		EndMutation:        aws_cryptography_keyStore_WriteMutatedVersionsInput_EndMutation_FromDafny(dafnyInput.Dtor_EndMutation()),
+	}
+
+}
+
+func WriteMutatedVersionsOutput_FromDafny(dafnyOutput AwsCryptographyKeyStoreTypes.WriteMutatedVersionsOutput) awscryptographykeystoresmithygeneratedtypes.WriteMutatedVersionsOutput {
+
+	return awscryptographykeystoresmithygeneratedtypes.WriteMutatedVersionsOutput{}
+
+}
+
+func WriteMutationIndexInput_FromDafny(dafnyInput AwsCryptographyKeyStoreTypes.WriteMutationIndexInput) awscryptographykeystoresmithygeneratedtypes.WriteMutationIndexInput {
+
+	return awscryptographykeystoresmithygeneratedtypes.WriteMutationIndexInput{MutationCommitment: aws_cryptography_keyStore_WriteMutationIndexInput_MutationCommitment_FromDafny(dafnyInput.Dtor_MutationCommitment()),
+		MutationIndex: aws_cryptography_keyStore_WriteMutationIndexInput_MutationIndex_FromDafny(dafnyInput.Dtor_MutationIndex()),
+	}
+
+}
+
+func WriteMutationIndexOutput_FromDafny(dafnyOutput AwsCryptographyKeyStoreTypes.WriteMutationIndexOutput) awscryptographykeystoresmithygeneratedtypes.WriteMutationIndexOutput {
+
+	return awscryptographykeystoresmithygeneratedtypes.WriteMutationIndexOutput{}
 
 }
 
@@ -181,8 +303,7 @@ func WriteNewEncryptedBranchKeyOutput_FromDafny(dafnyOutput AwsCryptographyKeySt
 func WriteNewEncryptedBranchKeyVersionInput_FromDafny(dafnyInput AwsCryptographyKeyStoreTypes.WriteNewEncryptedBranchKeyVersionInput) awscryptographykeystoresmithygeneratedtypes.WriteNewEncryptedBranchKeyVersionInput {
 
 	return awscryptographykeystoresmithygeneratedtypes.WriteNewEncryptedBranchKeyVersionInput{Active: aws_cryptography_keyStore_WriteNewEncryptedBranchKeyVersionInput_Active_FromDafny(dafnyInput.Dtor_Active()),
-		Version:   aws_cryptography_keyStore_WriteNewEncryptedBranchKeyVersionInput_Version_FromDafny(dafnyInput.Dtor_Version()),
-		OldActive: aws_cryptography_keyStore_WriteNewEncryptedBranchKeyVersionInput_oldActive_FromDafny(dafnyInput.Dtor_oldActive()),
+		Version: aws_cryptography_keyStore_WriteNewEncryptedBranchKeyVersionInput_Version_FromDafny(dafnyInput.Dtor_Version()),
 	}
 
 }
@@ -193,8 +314,43 @@ func WriteNewEncryptedBranchKeyVersionOutput_FromDafny(dafnyOutput AwsCryptograp
 
 }
 
+func AlreadyExistsConditionFailed_FromDafny(dafnyOutput AwsCryptographyKeyStoreTypes.Error) awscryptographykeystoresmithygeneratedtypes.AlreadyExistsConditionFailed {
+	return awscryptographykeystoresmithygeneratedtypes.AlreadyExistsConditionFailed{Message: aws_cryptography_keyStore_AlreadyExistsConditionFailed_message_FromDafny(dafnyOutput.Dtor_message())}
+
+}
+
+func KeyManagementException_FromDafny(dafnyOutput AwsCryptographyKeyStoreTypes.Error) awscryptographykeystoresmithygeneratedtypes.KeyManagementException {
+	return awscryptographykeystoresmithygeneratedtypes.KeyManagementException{Message: aws_cryptography_keyStore_KeyManagementException_message_FromDafny(dafnyOutput.Dtor_message())}
+
+}
+
+func KeyStorageException_FromDafny(dafnyOutput AwsCryptographyKeyStoreTypes.Error) awscryptographykeystoresmithygeneratedtypes.KeyStorageException {
+	return awscryptographykeystoresmithygeneratedtypes.KeyStorageException{Message: aws_cryptography_keyStore_KeyStorageException_message_FromDafny(dafnyOutput.Dtor_message())}
+
+}
+
 func KeyStoreException_FromDafny(dafnyOutput AwsCryptographyKeyStoreTypes.Error) awscryptographykeystoresmithygeneratedtypes.KeyStoreException {
 	return awscryptographykeystoresmithygeneratedtypes.KeyStoreException{Message: aws_cryptography_keyStore_KeyStoreException_message_FromDafny(dafnyOutput.Dtor_message())}
+
+}
+
+func MutationCommitmentConditionFailed_FromDafny(dafnyOutput AwsCryptographyKeyStoreTypes.Error) awscryptographykeystoresmithygeneratedtypes.MutationCommitmentConditionFailed {
+	return awscryptographykeystoresmithygeneratedtypes.MutationCommitmentConditionFailed{Message: aws_cryptography_keyStore_MutationCommitmentConditionFailed_message_FromDafny(dafnyOutput.Dtor_message())}
+
+}
+
+func NoLongerExistsConditionFailed_FromDafny(dafnyOutput AwsCryptographyKeyStoreTypes.Error) awscryptographykeystoresmithygeneratedtypes.NoLongerExistsConditionFailed {
+	return awscryptographykeystoresmithygeneratedtypes.NoLongerExistsConditionFailed{Message: aws_cryptography_keyStore_NoLongerExistsConditionFailed_message_FromDafny(dafnyOutput.Dtor_message())}
+
+}
+
+func OldEncConditionFailed_FromDafny(dafnyOutput AwsCryptographyKeyStoreTypes.Error) awscryptographykeystoresmithygeneratedtypes.OldEncConditionFailed {
+	return awscryptographykeystoresmithygeneratedtypes.OldEncConditionFailed{Message: aws_cryptography_keyStore_OldEncConditionFailed_message_FromDafny(dafnyOutput.Dtor_message())}
+
+}
+
+func VersionRaceException_FromDafny(dafnyOutput AwsCryptographyKeyStoreTypes.Error) awscryptographykeystoresmithygeneratedtypes.VersionRaceException {
+	return awscryptographykeystoresmithygeneratedtypes.VersionRaceException{Message: aws_cryptography_keyStore_VersionRaceException_message_FromDafny(dafnyOutput.Dtor_message())}
 
 }
 
@@ -232,8 +388,36 @@ func OpaqueError_Output_FromDafny(dafnyOutput AwsCryptographyKeyStoreTypes.Error
 
 func Error_FromDafny(err AwsCryptographyKeyStoreTypes.Error) error {
 	// Service Errors
+	if err.Is_AlreadyExistsConditionFailed() {
+		return AlreadyExistsConditionFailed_FromDafny(err)
+	}
+
+	if err.Is_KeyManagementException() {
+		return KeyManagementException_FromDafny(err)
+	}
+
+	if err.Is_KeyStorageException() {
+		return KeyStorageException_FromDafny(err)
+	}
+
 	if err.Is_KeyStoreException() {
 		return KeyStoreException_FromDafny(err)
+	}
+
+	if err.Is_MutationCommitmentConditionFailed() {
+		return MutationCommitmentConditionFailed_FromDafny(err)
+	}
+
+	if err.Is_NoLongerExistsConditionFailed() {
+		return NoLongerExistsConditionFailed_FromDafny(err)
+	}
+
+	if err.Is_OldEncConditionFailed() {
+		return OldEncConditionFailed_FromDafny(err)
+	}
+
+	if err.Is_VersionRaceException() {
+		return VersionRaceException_FromDafny(err)
 	}
 
 	//DependentErrors
@@ -280,6 +464,18 @@ func ActiveHierarchicalSymmetricBeacon_FromDafny(input interface{}) awscryptogra
 func AwsKms_FromDafny(input interface{}) awscryptographykeystoresmithygeneratedtypes.AwsKms {
 	return awscryptographykeystoresmithygeneratedtypes.AwsKms{GrantTokens: aws_cryptography_keyStore_AwsKms_grantTokens_FromDafny(input.(AwsCryptographyKeyStoreTypes.AwsKms).Dtor_grantTokens().UnwrapOr(nil)),
 		KmsClient: aws_cryptography_keyStore_AwsKms_kmsClient_FromDafny(input.(AwsCryptographyKeyStoreTypes.AwsKms).Dtor_kmsClient().UnwrapOr(nil)),
+	}
+
+}
+
+func MutationCommitment_FromDafny(input interface{}) awscryptographykeystoresmithygeneratedtypes.MutationCommitment {
+	return awscryptographykeystoresmithygeneratedtypes.MutationCommitment{Identifier: aws_cryptography_keyStore_MutationCommitment_Identifier_FromDafny(input.(AwsCryptographyKeyStoreTypes.MutationCommitment).Dtor_Identifier()),
+		CreateTime:     aws_cryptography_keyStore_MutationCommitment_CreateTime_FromDafny(input.(AwsCryptographyKeyStoreTypes.MutationCommitment).Dtor_CreateTime()),
+		UUID:           aws_cryptography_keyStore_MutationCommitment_UUID_FromDafny(input.(AwsCryptographyKeyStoreTypes.MutationCommitment).Dtor_UUID()),
+		Original:       aws_cryptography_keyStore_MutationCommitment_Original_FromDafny(input.(AwsCryptographyKeyStoreTypes.MutationCommitment).Dtor_Original()),
+		Terminal:       aws_cryptography_keyStore_MutationCommitment_Terminal_FromDafny(input.(AwsCryptographyKeyStoreTypes.MutationCommitment).Dtor_Terminal()),
+		Input:          aws_cryptography_keyStore_MutationCommitment_Input_FromDafny(input.(AwsCryptographyKeyStoreTypes.MutationCommitment).Dtor_Input()),
+		CiphertextBlob: aws_cryptography_keyStore_MutationCommitment_CiphertextBlob_FromDafny(input.(AwsCryptographyKeyStoreTypes.MutationCommitment).Dtor_CiphertextBlob()),
 	}
 
 }
@@ -333,6 +529,16 @@ func EncryptedHierarchicalKey_FromDafny(input interface{}) awscryptographykeysto
 
 }
 
+func MutationIndex_FromDafny(input interface{}) awscryptographykeystoresmithygeneratedtypes.MutationIndex {
+	return awscryptographykeystoresmithygeneratedtypes.MutationIndex{Identifier: aws_cryptography_keyStore_MutationIndex_Identifier_FromDafny(input.(AwsCryptographyKeyStoreTypes.MutationIndex).Dtor_Identifier()),
+		CreateTime:     aws_cryptography_keyStore_MutationIndex_CreateTime_FromDafny(input.(AwsCryptographyKeyStoreTypes.MutationIndex).Dtor_CreateTime()),
+		UUID:           aws_cryptography_keyStore_MutationIndex_UUID_FromDafny(input.(AwsCryptographyKeyStoreTypes.MutationIndex).Dtor_UUID()),
+		PageIndex:      aws_cryptography_keyStore_MutationIndex_PageIndex_FromDafny(input.(AwsCryptographyKeyStoreTypes.MutationIndex).Dtor_PageIndex()),
+		CiphertextBlob: aws_cryptography_keyStore_MutationIndex_CiphertextBlob_FromDafny(input.(AwsCryptographyKeyStoreTypes.MutationIndex).Dtor_CiphertextBlob()),
+	}
+
+}
+
 func KeyManagement_FromDafny(input interface{}) awscryptographykeystoresmithygeneratedtypes.KeyManagement {
 	var union awscryptographykeystoresmithygeneratedtypes.KeyManagement
 
@@ -344,6 +550,40 @@ func KeyManagement_FromDafny(input interface{}) awscryptographykeystoresmithygen
 	}
 
 	return union
+
+}
+
+func OverWriteEncryptedHierarchicalKey_FromDafny(input interface{}) awscryptographykeystoresmithygeneratedtypes.OverWriteEncryptedHierarchicalKey {
+	return awscryptographykeystoresmithygeneratedtypes.OverWriteEncryptedHierarchicalKey{Item: aws_cryptography_keyStore_OverWriteEncryptedHierarchicalKey_Item_FromDafny(input.(AwsCryptographyKeyStoreTypes.OverWriteEncryptedHierarchicalKey).Dtor_Item()),
+		Old: aws_cryptography_keyStore_OverWriteEncryptedHierarchicalKey_Old_FromDafny(input.(AwsCryptographyKeyStoreTypes.OverWriteEncryptedHierarchicalKey).Dtor_Old()),
+	}
+
+}
+
+func WriteInitializeMutationVersion_FromDafny(input interface{}) awscryptographykeystoresmithygeneratedtypes.WriteInitializeMutationVersion {
+	var union awscryptographykeystoresmithygeneratedtypes.WriteInitializeMutationVersion
+
+	if (input.(AwsCryptographyKeyStoreTypes.WriteInitializeMutationVersion)).Is_rotate() {
+
+		union = &awscryptographykeystoresmithygeneratedtypes.WriteInitializeMutationVersionMemberrotate{
+			Value: (aws_cryptography_keyStore_WriteInitializeMutationVersion_rotate_FromDafny((input.(AwsCryptographyKeyStoreTypes.WriteInitializeMutationVersion)).Dtor_rotate())),
+		}
+	}
+	if (input.(AwsCryptographyKeyStoreTypes.WriteInitializeMutationVersion)).Is_mutate() {
+
+		union = &awscryptographykeystoresmithygeneratedtypes.WriteInitializeMutationVersionMembermutate{
+			Value: (aws_cryptography_keyStore_WriteInitializeMutationVersion_mutate_FromDafny((input.(AwsCryptographyKeyStoreTypes.WriteInitializeMutationVersion)).Dtor_mutate())),
+		}
+	}
+
+	return union
+
+}
+
+func OverWriteMutationIndex_FromDafny(input interface{}) awscryptographykeystoresmithygeneratedtypes.OverWriteMutationIndex {
+	return awscryptographykeystoresmithygeneratedtypes.OverWriteMutationIndex{Index: aws_cryptography_keyStore_OverWriteMutationIndex_Index_FromDafny(input.(AwsCryptographyKeyStoreTypes.OverWriteMutationIndex).Dtor_Index()),
+		Old: aws_cryptography_keyStore_OverWriteMutationIndex_Old_FromDafny(input.(AwsCryptographyKeyStoreTypes.OverWriteMutationIndex).Dtor_Old()),
+	}
 
 }
 
@@ -838,6 +1078,119 @@ func aws_cryptography_keyStore_VersionKeyInput_branchKeyIdentifier_FromDafny(inp
 		}
 	}()
 }
+func aws_cryptography_keyStore_DeleteMutationInput_MutationCommitment_FromDafny(input interface{}) awscryptographykeystoresmithygeneratedtypes.MutationCommitment {
+	return awscryptographykeystoresmithygeneratedtypes.MutationCommitment{Identifier: aws_cryptography_keyStore_MutationCommitment_Identifier_FromDafny(input.(AwsCryptographyKeyStoreTypes.MutationCommitment).Dtor_Identifier()),
+		CreateTime:     aws_cryptography_keyStore_MutationCommitment_CreateTime_FromDafny(input.(AwsCryptographyKeyStoreTypes.MutationCommitment).Dtor_CreateTime()),
+		UUID:           aws_cryptography_keyStore_MutationCommitment_UUID_FromDafny(input.(AwsCryptographyKeyStoreTypes.MutationCommitment).Dtor_UUID()),
+		Original:       aws_cryptography_keyStore_MutationCommitment_Original_FromDafny(input.(AwsCryptographyKeyStoreTypes.MutationCommitment).Dtor_Original()),
+		Terminal:       aws_cryptography_keyStore_MutationCommitment_Terminal_FromDafny(input.(AwsCryptographyKeyStoreTypes.MutationCommitment).Dtor_Terminal()),
+		Input:          aws_cryptography_keyStore_MutationCommitment_Input_FromDafny(input.(AwsCryptographyKeyStoreTypes.MutationCommitment).Dtor_Input()),
+		CiphertextBlob: aws_cryptography_keyStore_MutationCommitment_CiphertextBlob_FromDafny(input.(AwsCryptographyKeyStoreTypes.MutationCommitment).Dtor_CiphertextBlob()),
+	}
+}
+func aws_cryptography_keyStore_MutationCommitment_Identifier_FromDafny(input interface{}) string {
+	return func() string {
+		var s string
+		for i := dafny.Iterate(input); ; {
+			val, ok := i()
+			if !ok {
+				return s
+			} else {
+				s = s + string(val.(dafny.Char))
+			}
+		}
+	}()
+}
+func aws_cryptography_keyStore_MutationCommitment_CreateTime_FromDafny(input interface{}) string {
+	return func() string {
+		var s string
+		for i := dafny.Iterate(input); ; {
+			val, ok := i()
+			if !ok {
+				return s
+			} else {
+				s = s + string(val.(dafny.Char))
+			}
+		}
+	}()
+}
+func aws_cryptography_keyStore_MutationCommitment_UUID_FromDafny(input interface{}) string {
+	return func() string {
+		var s string
+		for i := dafny.Iterate(input); ; {
+			val, ok := i()
+			if !ok {
+				return s
+			} else {
+				s = s + string(val.(dafny.Char))
+			}
+		}
+	}()
+}
+func aws_cryptography_keyStore_MutationCommitment_Original_FromDafny(input interface{}) []byte {
+	return func() []byte {
+		var b []byte
+		if input == nil {
+			return nil
+		}
+		for i := dafny.Iterate(input); ; {
+			val, ok := i()
+			if !ok {
+				return b
+			} else {
+				b = append(b, val.(byte))
+			}
+		}
+	}()
+}
+func aws_cryptography_keyStore_MutationCommitment_Terminal_FromDafny(input interface{}) []byte {
+	return func() []byte {
+		var b []byte
+		if input == nil {
+			return nil
+		}
+		for i := dafny.Iterate(input); ; {
+			val, ok := i()
+			if !ok {
+				return b
+			} else {
+				b = append(b, val.(byte))
+			}
+		}
+	}()
+}
+func aws_cryptography_keyStore_MutationCommitment_Input_FromDafny(input interface{}) []byte {
+	return func() []byte {
+		var b []byte
+		if input == nil {
+			return nil
+		}
+		for i := dafny.Iterate(input); ; {
+			val, ok := i()
+			if !ok {
+				return b
+			} else {
+				b = append(b, val.(byte))
+			}
+		}
+	}()
+}
+func aws_cryptography_keyStore_MutationCommitment_CiphertextBlob_FromDafny(input interface{}) []byte {
+	return func() []byte {
+		var b []byte
+		if input == nil {
+			return nil
+		}
+		for i := dafny.Iterate(input); ; {
+			val, ok := i()
+			if !ok {
+				return b
+			} else {
+				b = append(b, val.(byte))
+			}
+		}
+	}()
+}
 func aws_cryptography_keyStore_GetEncryptedActiveBranchKeyInput_Identifier_FromDafny(input interface{}) string {
 	return func() string {
 		var s string
@@ -1073,6 +1426,132 @@ func aws_cryptography_keyStore_GetEncryptedBranchKeyVersionOutput_Item_FromDafny
 		CiphertextBlob:    aws_cryptography_keyStore_EncryptedHierarchicalKey_CiphertextBlob_FromDafny(input.(AwsCryptographyKeyStoreTypes.EncryptedHierarchicalKey).Dtor_CiphertextBlob()),
 	}
 }
+func aws_cryptography_keyStore_GetItemsForInitializeMutationInput_Identifier_FromDafny(input interface{}) string {
+	return func() string {
+		var s string
+		for i := dafny.Iterate(input); ; {
+			val, ok := i()
+			if !ok {
+				return s
+			} else {
+				s = s + string(val.(dafny.Char))
+			}
+		}
+	}()
+}
+func aws_cryptography_keyStore_GetItemsForInitializeMutationOutput_ActiveItem_FromDafny(input interface{}) awscryptographykeystoresmithygeneratedtypes.EncryptedHierarchicalKey {
+	return awscryptographykeystoresmithygeneratedtypes.EncryptedHierarchicalKey{Identifier: aws_cryptography_keyStore_EncryptedHierarchicalKey_Identifier_FromDafny(input.(AwsCryptographyKeyStoreTypes.EncryptedHierarchicalKey).Dtor_Identifier()),
+		Type:              aws_cryptography_keyStore_EncryptedHierarchicalKey_Type_FromDafny(input.(AwsCryptographyKeyStoreTypes.EncryptedHierarchicalKey).Dtor_Type()),
+		CreateTime:        aws_cryptography_keyStore_EncryptedHierarchicalKey_CreateTime_FromDafny(input.(AwsCryptographyKeyStoreTypes.EncryptedHierarchicalKey).Dtor_CreateTime()),
+		KmsArn:            aws_cryptography_keyStore_EncryptedHierarchicalKey_KmsArn_FromDafny(input.(AwsCryptographyKeyStoreTypes.EncryptedHierarchicalKey).Dtor_KmsArn()),
+		EncryptionContext: aws_cryptography_keyStore_EncryptedHierarchicalKey_EncryptionContext_FromDafny(input.(AwsCryptographyKeyStoreTypes.EncryptedHierarchicalKey).Dtor_EncryptionContext()),
+		CiphertextBlob:    aws_cryptography_keyStore_EncryptedHierarchicalKey_CiphertextBlob_FromDafny(input.(AwsCryptographyKeyStoreTypes.EncryptedHierarchicalKey).Dtor_CiphertextBlob()),
+	}
+}
+func aws_cryptography_keyStore_GetItemsForInitializeMutationOutput_BeaconItem_FromDafny(input interface{}) awscryptographykeystoresmithygeneratedtypes.EncryptedHierarchicalKey {
+	return awscryptographykeystoresmithygeneratedtypes.EncryptedHierarchicalKey{Identifier: aws_cryptography_keyStore_EncryptedHierarchicalKey_Identifier_FromDafny(input.(AwsCryptographyKeyStoreTypes.EncryptedHierarchicalKey).Dtor_Identifier()),
+		Type:              aws_cryptography_keyStore_EncryptedHierarchicalKey_Type_FromDafny(input.(AwsCryptographyKeyStoreTypes.EncryptedHierarchicalKey).Dtor_Type()),
+		CreateTime:        aws_cryptography_keyStore_EncryptedHierarchicalKey_CreateTime_FromDafny(input.(AwsCryptographyKeyStoreTypes.EncryptedHierarchicalKey).Dtor_CreateTime()),
+		KmsArn:            aws_cryptography_keyStore_EncryptedHierarchicalKey_KmsArn_FromDafny(input.(AwsCryptographyKeyStoreTypes.EncryptedHierarchicalKey).Dtor_KmsArn()),
+		EncryptionContext: aws_cryptography_keyStore_EncryptedHierarchicalKey_EncryptionContext_FromDafny(input.(AwsCryptographyKeyStoreTypes.EncryptedHierarchicalKey).Dtor_EncryptionContext()),
+		CiphertextBlob:    aws_cryptography_keyStore_EncryptedHierarchicalKey_CiphertextBlob_FromDafny(input.(AwsCryptographyKeyStoreTypes.EncryptedHierarchicalKey).Dtor_CiphertextBlob()),
+	}
+}
+func aws_cryptography_keyStore_GetItemsForInitializeMutationOutput_MutationCommitment_FromDafny(input interface{}) *awscryptographykeystoresmithygeneratedtypes.MutationCommitment {
+	if input == nil {
+		return nil
+	}
+	return &awscryptographykeystoresmithygeneratedtypes.MutationCommitment{Identifier: aws_cryptography_keyStore_MutationCommitment_Identifier_FromDafny(input.(AwsCryptographyKeyStoreTypes.MutationCommitment).Dtor_Identifier()),
+		CreateTime:     aws_cryptography_keyStore_MutationCommitment_CreateTime_FromDafny(input.(AwsCryptographyKeyStoreTypes.MutationCommitment).Dtor_CreateTime()),
+		UUID:           aws_cryptography_keyStore_MutationCommitment_UUID_FromDafny(input.(AwsCryptographyKeyStoreTypes.MutationCommitment).Dtor_UUID()),
+		Original:       aws_cryptography_keyStore_MutationCommitment_Original_FromDafny(input.(AwsCryptographyKeyStoreTypes.MutationCommitment).Dtor_Original()),
+		Terminal:       aws_cryptography_keyStore_MutationCommitment_Terminal_FromDafny(input.(AwsCryptographyKeyStoreTypes.MutationCommitment).Dtor_Terminal()),
+		Input:          aws_cryptography_keyStore_MutationCommitment_Input_FromDafny(input.(AwsCryptographyKeyStoreTypes.MutationCommitment).Dtor_Input()),
+		CiphertextBlob: aws_cryptography_keyStore_MutationCommitment_CiphertextBlob_FromDafny(input.(AwsCryptographyKeyStoreTypes.MutationCommitment).Dtor_CiphertextBlob()),
+	}
+}
+func aws_cryptography_keyStore_GetItemsForInitializeMutationOutput_MutationIndex_FromDafny(input interface{}) *awscryptographykeystoresmithygeneratedtypes.MutationIndex {
+	if input == nil {
+		return nil
+	}
+	return &awscryptographykeystoresmithygeneratedtypes.MutationIndex{Identifier: aws_cryptography_keyStore_MutationIndex_Identifier_FromDafny(input.(AwsCryptographyKeyStoreTypes.MutationIndex).Dtor_Identifier()),
+		CreateTime:     aws_cryptography_keyStore_MutationIndex_CreateTime_FromDafny(input.(AwsCryptographyKeyStoreTypes.MutationIndex).Dtor_CreateTime()),
+		UUID:           aws_cryptography_keyStore_MutationIndex_UUID_FromDafny(input.(AwsCryptographyKeyStoreTypes.MutationIndex).Dtor_UUID()),
+		PageIndex:      aws_cryptography_keyStore_MutationIndex_PageIndex_FromDafny(input.(AwsCryptographyKeyStoreTypes.MutationIndex).Dtor_PageIndex()),
+		CiphertextBlob: aws_cryptography_keyStore_MutationIndex_CiphertextBlob_FromDafny(input.(AwsCryptographyKeyStoreTypes.MutationIndex).Dtor_CiphertextBlob()),
+	}
+}
+func aws_cryptography_keyStore_MutationIndex_Identifier_FromDafny(input interface{}) string {
+	return func() string {
+		var s string
+		for i := dafny.Iterate(input); ; {
+			val, ok := i()
+			if !ok {
+				return s
+			} else {
+				s = s + string(val.(dafny.Char))
+			}
+		}
+	}()
+}
+func aws_cryptography_keyStore_MutationIndex_CreateTime_FromDafny(input interface{}) string {
+	return func() string {
+		var s string
+		for i := dafny.Iterate(input); ; {
+			val, ok := i()
+			if !ok {
+				return s
+			} else {
+				s = s + string(val.(dafny.Char))
+			}
+		}
+	}()
+}
+func aws_cryptography_keyStore_MutationIndex_UUID_FromDafny(input interface{}) string {
+	return func() string {
+		var s string
+		for i := dafny.Iterate(input); ; {
+			val, ok := i()
+			if !ok {
+				return s
+			} else {
+				s = s + string(val.(dafny.Char))
+			}
+		}
+	}()
+}
+func aws_cryptography_keyStore_MutationIndex_PageIndex_FromDafny(input interface{}) []byte {
+	return func() []byte {
+		var b []byte
+		if input == nil {
+			return nil
+		}
+		for i := dafny.Iterate(input); ; {
+			val, ok := i()
+			if !ok {
+				return b
+			} else {
+				b = append(b, val.(byte))
+			}
+		}
+	}()
+}
+func aws_cryptography_keyStore_MutationIndex_CiphertextBlob_FromDafny(input interface{}) []byte {
+	return func() []byte {
+		var b []byte
+		if input == nil {
+			return nil
+		}
+		for i := dafny.Iterate(input); ; {
+			val, ok := i()
+			if !ok {
+				return b
+			} else {
+				b = append(b, val.(byte))
+			}
+		}
+	}()
+}
 func aws_cryptography_keyStore_GetKeyStorageInfoOutput_Name_FromDafny(input interface{}) string {
 	return func() string {
 		var s string
@@ -1111,6 +1590,301 @@ func aws_cryptography_keyStore_GetKeyStorageInfoOutput_LogicalName_FromDafny(inp
 		}
 	}()
 }
+func aws_cryptography_keyStore_GetMutationInput_Identifier_FromDafny(input interface{}) string {
+	return func() string {
+		var s string
+		for i := dafny.Iterate(input); ; {
+			val, ok := i()
+			if !ok {
+				return s
+			} else {
+				s = s + string(val.(dafny.Char))
+			}
+		}
+	}()
+}
+func aws_cryptography_keyStore_GetMutationOutput_MutationCommitment_FromDafny(input interface{}) *awscryptographykeystoresmithygeneratedtypes.MutationCommitment {
+	if input == nil {
+		return nil
+	}
+	return &awscryptographykeystoresmithygeneratedtypes.MutationCommitment{Identifier: aws_cryptography_keyStore_MutationCommitment_Identifier_FromDafny(input.(AwsCryptographyKeyStoreTypes.MutationCommitment).Dtor_Identifier()),
+		CreateTime:     aws_cryptography_keyStore_MutationCommitment_CreateTime_FromDafny(input.(AwsCryptographyKeyStoreTypes.MutationCommitment).Dtor_CreateTime()),
+		UUID:           aws_cryptography_keyStore_MutationCommitment_UUID_FromDafny(input.(AwsCryptographyKeyStoreTypes.MutationCommitment).Dtor_UUID()),
+		Original:       aws_cryptography_keyStore_MutationCommitment_Original_FromDafny(input.(AwsCryptographyKeyStoreTypes.MutationCommitment).Dtor_Original()),
+		Terminal:       aws_cryptography_keyStore_MutationCommitment_Terminal_FromDafny(input.(AwsCryptographyKeyStoreTypes.MutationCommitment).Dtor_Terminal()),
+		Input:          aws_cryptography_keyStore_MutationCommitment_Input_FromDafny(input.(AwsCryptographyKeyStoreTypes.MutationCommitment).Dtor_Input()),
+		CiphertextBlob: aws_cryptography_keyStore_MutationCommitment_CiphertextBlob_FromDafny(input.(AwsCryptographyKeyStoreTypes.MutationCommitment).Dtor_CiphertextBlob()),
+	}
+}
+func aws_cryptography_keyStore_GetMutationOutput_MutationIndex_FromDafny(input interface{}) *awscryptographykeystoresmithygeneratedtypes.MutationIndex {
+	if input == nil {
+		return nil
+	}
+	return &awscryptographykeystoresmithygeneratedtypes.MutationIndex{Identifier: aws_cryptography_keyStore_MutationIndex_Identifier_FromDafny(input.(AwsCryptographyKeyStoreTypes.MutationIndex).Dtor_Identifier()),
+		CreateTime:     aws_cryptography_keyStore_MutationIndex_CreateTime_FromDafny(input.(AwsCryptographyKeyStoreTypes.MutationIndex).Dtor_CreateTime()),
+		UUID:           aws_cryptography_keyStore_MutationIndex_UUID_FromDafny(input.(AwsCryptographyKeyStoreTypes.MutationIndex).Dtor_UUID()),
+		PageIndex:      aws_cryptography_keyStore_MutationIndex_PageIndex_FromDafny(input.(AwsCryptographyKeyStoreTypes.MutationIndex).Dtor_PageIndex()),
+		CiphertextBlob: aws_cryptography_keyStore_MutationIndex_CiphertextBlob_FromDafny(input.(AwsCryptographyKeyStoreTypes.MutationIndex).Dtor_CiphertextBlob()),
+	}
+}
+func aws_cryptography_keyStore_QueryForVersionsInput_ExclusiveStartKey_FromDafny(input interface{}) []byte {
+	return func() []byte {
+		var b []byte
+		if input == nil {
+			return nil
+		}
+		for i := dafny.Iterate(input); ; {
+			val, ok := i()
+			if !ok {
+				return b
+			} else {
+				b = append(b, val.(byte))
+			}
+		}
+	}()
+}
+func aws_cryptography_keyStore_QueryForVersionsInput_Identifier_FromDafny(input interface{}) string {
+	return func() string {
+		var s string
+		for i := dafny.Iterate(input); ; {
+			val, ok := i()
+			if !ok {
+				return s
+			} else {
+				s = s + string(val.(dafny.Char))
+			}
+		}
+	}()
+}
+func aws_cryptography_keyStore_QueryForVersionsInput_PageSize_FromDafny(input interface{}) int32 {
+	return func() int32 {
+		var b = input.(int32)
+		return b
+	}()
+}
+func aws_cryptography_keyStore_QueryForVersionsOutput_ExclusiveStartKey_FromDafny(input interface{}) []byte {
+	return func() []byte {
+		var b []byte
+		if input == nil {
+			return nil
+		}
+		for i := dafny.Iterate(input); ; {
+			val, ok := i()
+			if !ok {
+				return b
+			} else {
+				b = append(b, val.(byte))
+			}
+		}
+	}()
+}
+func aws_cryptography_keyStore_QueryForVersionsOutput_Items_FromDafny(input interface{}) []awscryptographykeystoresmithygeneratedtypes.EncryptedHierarchicalKey {
+	fieldValue := make([]awscryptographykeystoresmithygeneratedtypes.EncryptedHierarchicalKey, 0)
+	for i := dafny.Iterate(input.(dafny.Sequence)); ; {
+		val, ok := i()
+		if !ok {
+			break
+		}
+		fieldValue = append(fieldValue, aws_cryptography_keyStore_EncryptedHierarchicalKeys_member_FromDafny(val))
+	}
+	return fieldValue
+}
+func aws_cryptography_keyStore_EncryptedHierarchicalKeys_member_FromDafny(input interface{}) awscryptographykeystoresmithygeneratedtypes.EncryptedHierarchicalKey {
+	return awscryptographykeystoresmithygeneratedtypes.EncryptedHierarchicalKey{Identifier: aws_cryptography_keyStore_EncryptedHierarchicalKey_Identifier_FromDafny(input.(AwsCryptographyKeyStoreTypes.EncryptedHierarchicalKey).Dtor_Identifier()),
+		Type:              aws_cryptography_keyStore_EncryptedHierarchicalKey_Type_FromDafny(input.(AwsCryptographyKeyStoreTypes.EncryptedHierarchicalKey).Dtor_Type()),
+		CreateTime:        aws_cryptography_keyStore_EncryptedHierarchicalKey_CreateTime_FromDafny(input.(AwsCryptographyKeyStoreTypes.EncryptedHierarchicalKey).Dtor_CreateTime()),
+		KmsArn:            aws_cryptography_keyStore_EncryptedHierarchicalKey_KmsArn_FromDafny(input.(AwsCryptographyKeyStoreTypes.EncryptedHierarchicalKey).Dtor_KmsArn()),
+		EncryptionContext: aws_cryptography_keyStore_EncryptedHierarchicalKey_EncryptionContext_FromDafny(input.(AwsCryptographyKeyStoreTypes.EncryptedHierarchicalKey).Dtor_EncryptionContext()),
+		CiphertextBlob:    aws_cryptography_keyStore_EncryptedHierarchicalKey_CiphertextBlob_FromDafny(input.(AwsCryptographyKeyStoreTypes.EncryptedHierarchicalKey).Dtor_CiphertextBlob()),
+	}
+}
+func aws_cryptography_keyStore_WriteAtomicMutationInput_Active_FromDafny(input interface{}) awscryptographykeystoresmithygeneratedtypes.OverWriteEncryptedHierarchicalKey {
+	return awscryptographykeystoresmithygeneratedtypes.OverWriteEncryptedHierarchicalKey{Item: aws_cryptography_keyStore_OverWriteEncryptedHierarchicalKey_Item_FromDafny(input.(AwsCryptographyKeyStoreTypes.OverWriteEncryptedHierarchicalKey).Dtor_Item()),
+		Old: aws_cryptography_keyStore_OverWriteEncryptedHierarchicalKey_Old_FromDafny(input.(AwsCryptographyKeyStoreTypes.OverWriteEncryptedHierarchicalKey).Dtor_Old()),
+	}
+}
+func aws_cryptography_keyStore_OverWriteEncryptedHierarchicalKey_Item_FromDafny(input interface{}) awscryptographykeystoresmithygeneratedtypes.EncryptedHierarchicalKey {
+	return awscryptographykeystoresmithygeneratedtypes.EncryptedHierarchicalKey{Identifier: aws_cryptography_keyStore_EncryptedHierarchicalKey_Identifier_FromDafny(input.(AwsCryptographyKeyStoreTypes.EncryptedHierarchicalKey).Dtor_Identifier()),
+		Type:              aws_cryptography_keyStore_EncryptedHierarchicalKey_Type_FromDafny(input.(AwsCryptographyKeyStoreTypes.EncryptedHierarchicalKey).Dtor_Type()),
+		CreateTime:        aws_cryptography_keyStore_EncryptedHierarchicalKey_CreateTime_FromDafny(input.(AwsCryptographyKeyStoreTypes.EncryptedHierarchicalKey).Dtor_CreateTime()),
+		KmsArn:            aws_cryptography_keyStore_EncryptedHierarchicalKey_KmsArn_FromDafny(input.(AwsCryptographyKeyStoreTypes.EncryptedHierarchicalKey).Dtor_KmsArn()),
+		EncryptionContext: aws_cryptography_keyStore_EncryptedHierarchicalKey_EncryptionContext_FromDafny(input.(AwsCryptographyKeyStoreTypes.EncryptedHierarchicalKey).Dtor_EncryptionContext()),
+		CiphertextBlob:    aws_cryptography_keyStore_EncryptedHierarchicalKey_CiphertextBlob_FromDafny(input.(AwsCryptographyKeyStoreTypes.EncryptedHierarchicalKey).Dtor_CiphertextBlob()),
+	}
+}
+func aws_cryptography_keyStore_OverWriteEncryptedHierarchicalKey_Old_FromDafny(input interface{}) awscryptographykeystoresmithygeneratedtypes.EncryptedHierarchicalKey {
+	return awscryptographykeystoresmithygeneratedtypes.EncryptedHierarchicalKey{Identifier: aws_cryptography_keyStore_EncryptedHierarchicalKey_Identifier_FromDafny(input.(AwsCryptographyKeyStoreTypes.EncryptedHierarchicalKey).Dtor_Identifier()),
+		Type:              aws_cryptography_keyStore_EncryptedHierarchicalKey_Type_FromDafny(input.(AwsCryptographyKeyStoreTypes.EncryptedHierarchicalKey).Dtor_Type()),
+		CreateTime:        aws_cryptography_keyStore_EncryptedHierarchicalKey_CreateTime_FromDafny(input.(AwsCryptographyKeyStoreTypes.EncryptedHierarchicalKey).Dtor_CreateTime()),
+		KmsArn:            aws_cryptography_keyStore_EncryptedHierarchicalKey_KmsArn_FromDafny(input.(AwsCryptographyKeyStoreTypes.EncryptedHierarchicalKey).Dtor_KmsArn()),
+		EncryptionContext: aws_cryptography_keyStore_EncryptedHierarchicalKey_EncryptionContext_FromDafny(input.(AwsCryptographyKeyStoreTypes.EncryptedHierarchicalKey).Dtor_EncryptionContext()),
+		CiphertextBlob:    aws_cryptography_keyStore_EncryptedHierarchicalKey_CiphertextBlob_FromDafny(input.(AwsCryptographyKeyStoreTypes.EncryptedHierarchicalKey).Dtor_CiphertextBlob()),
+	}
+}
+func aws_cryptography_keyStore_WriteAtomicMutationInput_Version_FromDafny(input interface{}) awscryptographykeystoresmithygeneratedtypes.WriteInitializeMutationVersion {
+	var union awscryptographykeystoresmithygeneratedtypes.WriteInitializeMutationVersion
+
+	if (input.(AwsCryptographyKeyStoreTypes.WriteInitializeMutationVersion)).Is_rotate() {
+
+		union = &awscryptographykeystoresmithygeneratedtypes.WriteInitializeMutationVersionMemberrotate{
+			Value: (aws_cryptography_keyStore_WriteInitializeMutationVersion_rotate_FromDafny((input.(AwsCryptographyKeyStoreTypes.WriteInitializeMutationVersion)).Dtor_rotate())),
+		}
+	}
+	if (input.(AwsCryptographyKeyStoreTypes.WriteInitializeMutationVersion)).Is_mutate() {
+
+		union = &awscryptographykeystoresmithygeneratedtypes.WriteInitializeMutationVersionMembermutate{
+			Value: (aws_cryptography_keyStore_WriteInitializeMutationVersion_mutate_FromDafny((input.(AwsCryptographyKeyStoreTypes.WriteInitializeMutationVersion)).Dtor_mutate())),
+		}
+	}
+
+	return union
+
+}
+func aws_cryptography_keyStore_WriteInitializeMutationVersion_rotate_FromDafny(input interface{}) awscryptographykeystoresmithygeneratedtypes.EncryptedHierarchicalKey {
+	return awscryptographykeystoresmithygeneratedtypes.EncryptedHierarchicalKey{Identifier: aws_cryptography_keyStore_EncryptedHierarchicalKey_Identifier_FromDafny(input.(AwsCryptographyKeyStoreTypes.EncryptedHierarchicalKey).Dtor_Identifier()),
+		Type:              aws_cryptography_keyStore_EncryptedHierarchicalKey_Type_FromDafny(input.(AwsCryptographyKeyStoreTypes.EncryptedHierarchicalKey).Dtor_Type()),
+		CreateTime:        aws_cryptography_keyStore_EncryptedHierarchicalKey_CreateTime_FromDafny(input.(AwsCryptographyKeyStoreTypes.EncryptedHierarchicalKey).Dtor_CreateTime()),
+		KmsArn:            aws_cryptography_keyStore_EncryptedHierarchicalKey_KmsArn_FromDafny(input.(AwsCryptographyKeyStoreTypes.EncryptedHierarchicalKey).Dtor_KmsArn()),
+		EncryptionContext: aws_cryptography_keyStore_EncryptedHierarchicalKey_EncryptionContext_FromDafny(input.(AwsCryptographyKeyStoreTypes.EncryptedHierarchicalKey).Dtor_EncryptionContext()),
+		CiphertextBlob:    aws_cryptography_keyStore_EncryptedHierarchicalKey_CiphertextBlob_FromDafny(input.(AwsCryptographyKeyStoreTypes.EncryptedHierarchicalKey).Dtor_CiphertextBlob()),
+	}
+}
+func aws_cryptography_keyStore_WriteInitializeMutationVersion_mutate_FromDafny(input interface{}) awscryptographykeystoresmithygeneratedtypes.OverWriteEncryptedHierarchicalKey {
+	return awscryptographykeystoresmithygeneratedtypes.OverWriteEncryptedHierarchicalKey{Item: aws_cryptography_keyStore_OverWriteEncryptedHierarchicalKey_Item_FromDafny(input.(AwsCryptographyKeyStoreTypes.OverWriteEncryptedHierarchicalKey).Dtor_Item()),
+		Old: aws_cryptography_keyStore_OverWriteEncryptedHierarchicalKey_Old_FromDafny(input.(AwsCryptographyKeyStoreTypes.OverWriteEncryptedHierarchicalKey).Dtor_Old()),
+	}
+}
+func aws_cryptography_keyStore_WriteAtomicMutationInput_Beacon_FromDafny(input interface{}) awscryptographykeystoresmithygeneratedtypes.OverWriteEncryptedHierarchicalKey {
+	return awscryptographykeystoresmithygeneratedtypes.OverWriteEncryptedHierarchicalKey{Item: aws_cryptography_keyStore_OverWriteEncryptedHierarchicalKey_Item_FromDafny(input.(AwsCryptographyKeyStoreTypes.OverWriteEncryptedHierarchicalKey).Dtor_Item()),
+		Old: aws_cryptography_keyStore_OverWriteEncryptedHierarchicalKey_Old_FromDafny(input.(AwsCryptographyKeyStoreTypes.OverWriteEncryptedHierarchicalKey).Dtor_Old()),
+	}
+}
+func aws_cryptography_keyStore_WriteAtomicMutationInput_Items_FromDafny(input interface{}) []awscryptographykeystoresmithygeneratedtypes.OverWriteEncryptedHierarchicalKey {
+	fieldValue := make([]awscryptographykeystoresmithygeneratedtypes.OverWriteEncryptedHierarchicalKey, 0)
+	for i := dafny.Iterate(input.(dafny.Sequence)); ; {
+		val, ok := i()
+		if !ok {
+			break
+		}
+		fieldValue = append(fieldValue, aws_cryptography_keyStore_OverWriteEncryptedHierarchicalKeys_member_FromDafny(val))
+	}
+	return fieldValue
+}
+func aws_cryptography_keyStore_OverWriteEncryptedHierarchicalKeys_member_FromDafny(input interface{}) awscryptographykeystoresmithygeneratedtypes.OverWriteEncryptedHierarchicalKey {
+	return awscryptographykeystoresmithygeneratedtypes.OverWriteEncryptedHierarchicalKey{Item: aws_cryptography_keyStore_OverWriteEncryptedHierarchicalKey_Item_FromDafny(input.(AwsCryptographyKeyStoreTypes.OverWriteEncryptedHierarchicalKey).Dtor_Item()),
+		Old: aws_cryptography_keyStore_OverWriteEncryptedHierarchicalKey_Old_FromDafny(input.(AwsCryptographyKeyStoreTypes.OverWriteEncryptedHierarchicalKey).Dtor_Old()),
+	}
+}
+func aws_cryptography_keyStore_WriteInitializeMutationInput_Active_FromDafny(input interface{}) awscryptographykeystoresmithygeneratedtypes.OverWriteEncryptedHierarchicalKey {
+	return awscryptographykeystoresmithygeneratedtypes.OverWriteEncryptedHierarchicalKey{Item: aws_cryptography_keyStore_OverWriteEncryptedHierarchicalKey_Item_FromDafny(input.(AwsCryptographyKeyStoreTypes.OverWriteEncryptedHierarchicalKey).Dtor_Item()),
+		Old: aws_cryptography_keyStore_OverWriteEncryptedHierarchicalKey_Old_FromDafny(input.(AwsCryptographyKeyStoreTypes.OverWriteEncryptedHierarchicalKey).Dtor_Old()),
+	}
+}
+func aws_cryptography_keyStore_WriteInitializeMutationInput_Version_FromDafny(input interface{}) awscryptographykeystoresmithygeneratedtypes.WriteInitializeMutationVersion {
+	var union awscryptographykeystoresmithygeneratedtypes.WriteInitializeMutationVersion
+
+	if (input.(AwsCryptographyKeyStoreTypes.WriteInitializeMutationVersion)).Is_rotate() {
+
+		union = &awscryptographykeystoresmithygeneratedtypes.WriteInitializeMutationVersionMemberrotate{
+			Value: (aws_cryptography_keyStore_WriteInitializeMutationVersion_rotate_FromDafny((input.(AwsCryptographyKeyStoreTypes.WriteInitializeMutationVersion)).Dtor_rotate())),
+		}
+	}
+	if (input.(AwsCryptographyKeyStoreTypes.WriteInitializeMutationVersion)).Is_mutate() {
+
+		union = &awscryptographykeystoresmithygeneratedtypes.WriteInitializeMutationVersionMembermutate{
+			Value: (aws_cryptography_keyStore_WriteInitializeMutationVersion_mutate_FromDafny((input.(AwsCryptographyKeyStoreTypes.WriteInitializeMutationVersion)).Dtor_mutate())),
+		}
+	}
+
+	return union
+
+}
+func aws_cryptography_keyStore_WriteInitializeMutationInput_Beacon_FromDafny(input interface{}) awscryptographykeystoresmithygeneratedtypes.OverWriteEncryptedHierarchicalKey {
+	return awscryptographykeystoresmithygeneratedtypes.OverWriteEncryptedHierarchicalKey{Item: aws_cryptography_keyStore_OverWriteEncryptedHierarchicalKey_Item_FromDafny(input.(AwsCryptographyKeyStoreTypes.OverWriteEncryptedHierarchicalKey).Dtor_Item()),
+		Old: aws_cryptography_keyStore_OverWriteEncryptedHierarchicalKey_Old_FromDafny(input.(AwsCryptographyKeyStoreTypes.OverWriteEncryptedHierarchicalKey).Dtor_Old()),
+	}
+}
+func aws_cryptography_keyStore_WriteInitializeMutationInput_MutationCommitment_FromDafny(input interface{}) awscryptographykeystoresmithygeneratedtypes.MutationCommitment {
+	return awscryptographykeystoresmithygeneratedtypes.MutationCommitment{Identifier: aws_cryptography_keyStore_MutationCommitment_Identifier_FromDafny(input.(AwsCryptographyKeyStoreTypes.MutationCommitment).Dtor_Identifier()),
+		CreateTime:     aws_cryptography_keyStore_MutationCommitment_CreateTime_FromDafny(input.(AwsCryptographyKeyStoreTypes.MutationCommitment).Dtor_CreateTime()),
+		UUID:           aws_cryptography_keyStore_MutationCommitment_UUID_FromDafny(input.(AwsCryptographyKeyStoreTypes.MutationCommitment).Dtor_UUID()),
+		Original:       aws_cryptography_keyStore_MutationCommitment_Original_FromDafny(input.(AwsCryptographyKeyStoreTypes.MutationCommitment).Dtor_Original()),
+		Terminal:       aws_cryptography_keyStore_MutationCommitment_Terminal_FromDafny(input.(AwsCryptographyKeyStoreTypes.MutationCommitment).Dtor_Terminal()),
+		Input:          aws_cryptography_keyStore_MutationCommitment_Input_FromDafny(input.(AwsCryptographyKeyStoreTypes.MutationCommitment).Dtor_Input()),
+		CiphertextBlob: aws_cryptography_keyStore_MutationCommitment_CiphertextBlob_FromDafny(input.(AwsCryptographyKeyStoreTypes.MutationCommitment).Dtor_CiphertextBlob()),
+	}
+}
+func aws_cryptography_keyStore_WriteInitializeMutationInput_MutationIndex_FromDafny(input interface{}) awscryptographykeystoresmithygeneratedtypes.MutationIndex {
+	return awscryptographykeystoresmithygeneratedtypes.MutationIndex{Identifier: aws_cryptography_keyStore_MutationIndex_Identifier_FromDafny(input.(AwsCryptographyKeyStoreTypes.MutationIndex).Dtor_Identifier()),
+		CreateTime:     aws_cryptography_keyStore_MutationIndex_CreateTime_FromDafny(input.(AwsCryptographyKeyStoreTypes.MutationIndex).Dtor_CreateTime()),
+		UUID:           aws_cryptography_keyStore_MutationIndex_UUID_FromDafny(input.(AwsCryptographyKeyStoreTypes.MutationIndex).Dtor_UUID()),
+		PageIndex:      aws_cryptography_keyStore_MutationIndex_PageIndex_FromDafny(input.(AwsCryptographyKeyStoreTypes.MutationIndex).Dtor_PageIndex()),
+		CiphertextBlob: aws_cryptography_keyStore_MutationIndex_CiphertextBlob_FromDafny(input.(AwsCryptographyKeyStoreTypes.MutationIndex).Dtor_CiphertextBlob()),
+	}
+}
+func aws_cryptography_keyStore_WriteMutatedVersionsInput_Items_FromDafny(input interface{}) []awscryptographykeystoresmithygeneratedtypes.OverWriteEncryptedHierarchicalKey {
+	fieldValue := make([]awscryptographykeystoresmithygeneratedtypes.OverWriteEncryptedHierarchicalKey, 0)
+	for i := dafny.Iterate(input.(dafny.Sequence)); ; {
+		val, ok := i()
+		if !ok {
+			break
+		}
+		fieldValue = append(fieldValue, aws_cryptography_keyStore_OverWriteEncryptedHierarchicalKeys_member_FromDafny(val))
+	}
+	return fieldValue
+}
+func aws_cryptography_keyStore_WriteMutatedVersionsInput_MutationCommitment_FromDafny(input interface{}) awscryptographykeystoresmithygeneratedtypes.MutationCommitment {
+	return awscryptographykeystoresmithygeneratedtypes.MutationCommitment{Identifier: aws_cryptography_keyStore_MutationCommitment_Identifier_FromDafny(input.(AwsCryptographyKeyStoreTypes.MutationCommitment).Dtor_Identifier()),
+		CreateTime:     aws_cryptography_keyStore_MutationCommitment_CreateTime_FromDafny(input.(AwsCryptographyKeyStoreTypes.MutationCommitment).Dtor_CreateTime()),
+		UUID:           aws_cryptography_keyStore_MutationCommitment_UUID_FromDafny(input.(AwsCryptographyKeyStoreTypes.MutationCommitment).Dtor_UUID()),
+		Original:       aws_cryptography_keyStore_MutationCommitment_Original_FromDafny(input.(AwsCryptographyKeyStoreTypes.MutationCommitment).Dtor_Original()),
+		Terminal:       aws_cryptography_keyStore_MutationCommitment_Terminal_FromDafny(input.(AwsCryptographyKeyStoreTypes.MutationCommitment).Dtor_Terminal()),
+		Input:          aws_cryptography_keyStore_MutationCommitment_Input_FromDafny(input.(AwsCryptographyKeyStoreTypes.MutationCommitment).Dtor_Input()),
+		CiphertextBlob: aws_cryptography_keyStore_MutationCommitment_CiphertextBlob_FromDafny(input.(AwsCryptographyKeyStoreTypes.MutationCommitment).Dtor_CiphertextBlob()),
+	}
+}
+func aws_cryptography_keyStore_WriteMutatedVersionsInput_MutationIndex_FromDafny(input interface{}) awscryptographykeystoresmithygeneratedtypes.OverWriteMutationIndex {
+	return awscryptographykeystoresmithygeneratedtypes.OverWriteMutationIndex{Index: aws_cryptography_keyStore_OverWriteMutationIndex_Index_FromDafny(input.(AwsCryptographyKeyStoreTypes.OverWriteMutationIndex).Dtor_Index()),
+		Old: aws_cryptography_keyStore_OverWriteMutationIndex_Old_FromDafny(input.(AwsCryptographyKeyStoreTypes.OverWriteMutationIndex).Dtor_Old()),
+	}
+}
+func aws_cryptography_keyStore_OverWriteMutationIndex_Index_FromDafny(input interface{}) awscryptographykeystoresmithygeneratedtypes.MutationIndex {
+	return awscryptographykeystoresmithygeneratedtypes.MutationIndex{Identifier: aws_cryptography_keyStore_MutationIndex_Identifier_FromDafny(input.(AwsCryptographyKeyStoreTypes.MutationIndex).Dtor_Identifier()),
+		CreateTime:     aws_cryptography_keyStore_MutationIndex_CreateTime_FromDafny(input.(AwsCryptographyKeyStoreTypes.MutationIndex).Dtor_CreateTime()),
+		UUID:           aws_cryptography_keyStore_MutationIndex_UUID_FromDafny(input.(AwsCryptographyKeyStoreTypes.MutationIndex).Dtor_UUID()),
+		PageIndex:      aws_cryptography_keyStore_MutationIndex_PageIndex_FromDafny(input.(AwsCryptographyKeyStoreTypes.MutationIndex).Dtor_PageIndex()),
+		CiphertextBlob: aws_cryptography_keyStore_MutationIndex_CiphertextBlob_FromDafny(input.(AwsCryptographyKeyStoreTypes.MutationIndex).Dtor_CiphertextBlob()),
+	}
+}
+func aws_cryptography_keyStore_OverWriteMutationIndex_Old_FromDafny(input interface{}) awscryptographykeystoresmithygeneratedtypes.MutationIndex {
+	return awscryptographykeystoresmithygeneratedtypes.MutationIndex{Identifier: aws_cryptography_keyStore_MutationIndex_Identifier_FromDafny(input.(AwsCryptographyKeyStoreTypes.MutationIndex).Dtor_Identifier()),
+		CreateTime:     aws_cryptography_keyStore_MutationIndex_CreateTime_FromDafny(input.(AwsCryptographyKeyStoreTypes.MutationIndex).Dtor_CreateTime()),
+		UUID:           aws_cryptography_keyStore_MutationIndex_UUID_FromDafny(input.(AwsCryptographyKeyStoreTypes.MutationIndex).Dtor_UUID()),
+		PageIndex:      aws_cryptography_keyStore_MutationIndex_PageIndex_FromDafny(input.(AwsCryptographyKeyStoreTypes.MutationIndex).Dtor_PageIndex()),
+		CiphertextBlob: aws_cryptography_keyStore_MutationIndex_CiphertextBlob_FromDafny(input.(AwsCryptographyKeyStoreTypes.MutationIndex).Dtor_CiphertextBlob()),
+	}
+}
+func aws_cryptography_keyStore_WriteMutatedVersionsInput_EndMutation_FromDafny(input interface{}) bool {
+	return input.(bool)
+}
+func aws_cryptography_keyStore_WriteMutationIndexInput_MutationCommitment_FromDafny(input interface{}) awscryptographykeystoresmithygeneratedtypes.MutationCommitment {
+	return awscryptographykeystoresmithygeneratedtypes.MutationCommitment{Identifier: aws_cryptography_keyStore_MutationCommitment_Identifier_FromDafny(input.(AwsCryptographyKeyStoreTypes.MutationCommitment).Dtor_Identifier()),
+		CreateTime:     aws_cryptography_keyStore_MutationCommitment_CreateTime_FromDafny(input.(AwsCryptographyKeyStoreTypes.MutationCommitment).Dtor_CreateTime()),
+		UUID:           aws_cryptography_keyStore_MutationCommitment_UUID_FromDafny(input.(AwsCryptographyKeyStoreTypes.MutationCommitment).Dtor_UUID()),
+		Original:       aws_cryptography_keyStore_MutationCommitment_Original_FromDafny(input.(AwsCryptographyKeyStoreTypes.MutationCommitment).Dtor_Original()),
+		Terminal:       aws_cryptography_keyStore_MutationCommitment_Terminal_FromDafny(input.(AwsCryptographyKeyStoreTypes.MutationCommitment).Dtor_Terminal()),
+		Input:          aws_cryptography_keyStore_MutationCommitment_Input_FromDafny(input.(AwsCryptographyKeyStoreTypes.MutationCommitment).Dtor_Input()),
+		CiphertextBlob: aws_cryptography_keyStore_MutationCommitment_CiphertextBlob_FromDafny(input.(AwsCryptographyKeyStoreTypes.MutationCommitment).Dtor_CiphertextBlob()),
+	}
+}
+func aws_cryptography_keyStore_WriteMutationIndexInput_MutationIndex_FromDafny(input interface{}) awscryptographykeystoresmithygeneratedtypes.MutationIndex {
+	return awscryptographykeystoresmithygeneratedtypes.MutationIndex{Identifier: aws_cryptography_keyStore_MutationIndex_Identifier_FromDafny(input.(AwsCryptographyKeyStoreTypes.MutationIndex).Dtor_Identifier()),
+		CreateTime:     aws_cryptography_keyStore_MutationIndex_CreateTime_FromDafny(input.(AwsCryptographyKeyStoreTypes.MutationIndex).Dtor_CreateTime()),
+		UUID:           aws_cryptography_keyStore_MutationIndex_UUID_FromDafny(input.(AwsCryptographyKeyStoreTypes.MutationIndex).Dtor_UUID()),
+		PageIndex:      aws_cryptography_keyStore_MutationIndex_PageIndex_FromDafny(input.(AwsCryptographyKeyStoreTypes.MutationIndex).Dtor_PageIndex()),
+		CiphertextBlob: aws_cryptography_keyStore_MutationIndex_CiphertextBlob_FromDafny(input.(AwsCryptographyKeyStoreTypes.MutationIndex).Dtor_CiphertextBlob()),
+	}
+}
 func aws_cryptography_keyStore_WriteNewEncryptedBranchKeyInput_Active_FromDafny(input interface{}) awscryptographykeystoresmithygeneratedtypes.EncryptedHierarchicalKey {
 	return awscryptographykeystoresmithygeneratedtypes.EncryptedHierarchicalKey{Identifier: aws_cryptography_keyStore_EncryptedHierarchicalKey_Identifier_FromDafny(input.(AwsCryptographyKeyStoreTypes.EncryptedHierarchicalKey).Dtor_Identifier()),
 		Type:              aws_cryptography_keyStore_EncryptedHierarchicalKey_Type_FromDafny(input.(AwsCryptographyKeyStoreTypes.EncryptedHierarchicalKey).Dtor_Type()),
@@ -1138,13 +1912,9 @@ func aws_cryptography_keyStore_WriteNewEncryptedBranchKeyInput_Beacon_FromDafny(
 		CiphertextBlob:    aws_cryptography_keyStore_EncryptedHierarchicalKey_CiphertextBlob_FromDafny(input.(AwsCryptographyKeyStoreTypes.EncryptedHierarchicalKey).Dtor_CiphertextBlob()),
 	}
 }
-func aws_cryptography_keyStore_WriteNewEncryptedBranchKeyVersionInput_Active_FromDafny(input interface{}) awscryptographykeystoresmithygeneratedtypes.EncryptedHierarchicalKey {
-	return awscryptographykeystoresmithygeneratedtypes.EncryptedHierarchicalKey{Identifier: aws_cryptography_keyStore_EncryptedHierarchicalKey_Identifier_FromDafny(input.(AwsCryptographyKeyStoreTypes.EncryptedHierarchicalKey).Dtor_Identifier()),
-		Type:              aws_cryptography_keyStore_EncryptedHierarchicalKey_Type_FromDafny(input.(AwsCryptographyKeyStoreTypes.EncryptedHierarchicalKey).Dtor_Type()),
-		CreateTime:        aws_cryptography_keyStore_EncryptedHierarchicalKey_CreateTime_FromDafny(input.(AwsCryptographyKeyStoreTypes.EncryptedHierarchicalKey).Dtor_CreateTime()),
-		KmsArn:            aws_cryptography_keyStore_EncryptedHierarchicalKey_KmsArn_FromDafny(input.(AwsCryptographyKeyStoreTypes.EncryptedHierarchicalKey).Dtor_KmsArn()),
-		EncryptionContext: aws_cryptography_keyStore_EncryptedHierarchicalKey_EncryptionContext_FromDafny(input.(AwsCryptographyKeyStoreTypes.EncryptedHierarchicalKey).Dtor_EncryptionContext()),
-		CiphertextBlob:    aws_cryptography_keyStore_EncryptedHierarchicalKey_CiphertextBlob_FromDafny(input.(AwsCryptographyKeyStoreTypes.EncryptedHierarchicalKey).Dtor_CiphertextBlob()),
+func aws_cryptography_keyStore_WriteNewEncryptedBranchKeyVersionInput_Active_FromDafny(input interface{}) awscryptographykeystoresmithygeneratedtypes.OverWriteEncryptedHierarchicalKey {
+	return awscryptographykeystoresmithygeneratedtypes.OverWriteEncryptedHierarchicalKey{Item: aws_cryptography_keyStore_OverWriteEncryptedHierarchicalKey_Item_FromDafny(input.(AwsCryptographyKeyStoreTypes.OverWriteEncryptedHierarchicalKey).Dtor_Item()),
+		Old: aws_cryptography_keyStore_OverWriteEncryptedHierarchicalKey_Old_FromDafny(input.(AwsCryptographyKeyStoreTypes.OverWriteEncryptedHierarchicalKey).Dtor_Old()),
 	}
 }
 func aws_cryptography_keyStore_WriteNewEncryptedBranchKeyVersionInput_Version_FromDafny(input interface{}) awscryptographykeystoresmithygeneratedtypes.EncryptedHierarchicalKey {
@@ -1156,16 +1926,98 @@ func aws_cryptography_keyStore_WriteNewEncryptedBranchKeyVersionInput_Version_Fr
 		CiphertextBlob:    aws_cryptography_keyStore_EncryptedHierarchicalKey_CiphertextBlob_FromDafny(input.(AwsCryptographyKeyStoreTypes.EncryptedHierarchicalKey).Dtor_CiphertextBlob()),
 	}
 }
-func aws_cryptography_keyStore_WriteNewEncryptedBranchKeyVersionInput_oldActive_FromDafny(input interface{}) awscryptographykeystoresmithygeneratedtypes.EncryptedHierarchicalKey {
-	return awscryptographykeystoresmithygeneratedtypes.EncryptedHierarchicalKey{Identifier: aws_cryptography_keyStore_EncryptedHierarchicalKey_Identifier_FromDafny(input.(AwsCryptographyKeyStoreTypes.EncryptedHierarchicalKey).Dtor_Identifier()),
-		Type:              aws_cryptography_keyStore_EncryptedHierarchicalKey_Type_FromDafny(input.(AwsCryptographyKeyStoreTypes.EncryptedHierarchicalKey).Dtor_Type()),
-		CreateTime:        aws_cryptography_keyStore_EncryptedHierarchicalKey_CreateTime_FromDafny(input.(AwsCryptographyKeyStoreTypes.EncryptedHierarchicalKey).Dtor_CreateTime()),
-		KmsArn:            aws_cryptography_keyStore_EncryptedHierarchicalKey_KmsArn_FromDafny(input.(AwsCryptographyKeyStoreTypes.EncryptedHierarchicalKey).Dtor_KmsArn()),
-		EncryptionContext: aws_cryptography_keyStore_EncryptedHierarchicalKey_EncryptionContext_FromDafny(input.(AwsCryptographyKeyStoreTypes.EncryptedHierarchicalKey).Dtor_EncryptionContext()),
-		CiphertextBlob:    aws_cryptography_keyStore_EncryptedHierarchicalKey_CiphertextBlob_FromDafny(input.(AwsCryptographyKeyStoreTypes.EncryptedHierarchicalKey).Dtor_CiphertextBlob()),
-	}
+func aws_cryptography_keyStore_AlreadyExistsConditionFailed_message_FromDafny(input interface{}) string {
+	return func() string {
+		var s string
+		for i := dafny.Iterate(input); ; {
+			val, ok := i()
+			if !ok {
+				return s
+			} else {
+				s = s + string(val.(dafny.Char))
+			}
+		}
+	}()
+}
+func aws_cryptography_keyStore_KeyManagementException_message_FromDafny(input interface{}) string {
+	return func() string {
+		var s string
+		for i := dafny.Iterate(input); ; {
+			val, ok := i()
+			if !ok {
+				return s
+			} else {
+				s = s + string(val.(dafny.Char))
+			}
+		}
+	}()
+}
+func aws_cryptography_keyStore_KeyStorageException_message_FromDafny(input interface{}) string {
+	return func() string {
+		var s string
+		for i := dafny.Iterate(input); ; {
+			val, ok := i()
+			if !ok {
+				return s
+			} else {
+				s = s + string(val.(dafny.Char))
+			}
+		}
+	}()
 }
 func aws_cryptography_keyStore_KeyStoreException_message_FromDafny(input interface{}) string {
+	return func() string {
+		var s string
+		for i := dafny.Iterate(input); ; {
+			val, ok := i()
+			if !ok {
+				return s
+			} else {
+				s = s + string(val.(dafny.Char))
+			}
+		}
+	}()
+}
+func aws_cryptography_keyStore_MutationCommitmentConditionFailed_message_FromDafny(input interface{}) string {
+	return func() string {
+		var s string
+		for i := dafny.Iterate(input); ; {
+			val, ok := i()
+			if !ok {
+				return s
+			} else {
+				s = s + string(val.(dafny.Char))
+			}
+		}
+	}()
+}
+func aws_cryptography_keyStore_NoLongerExistsConditionFailed_message_FromDafny(input interface{}) string {
+	return func() string {
+		var s string
+		for i := dafny.Iterate(input); ; {
+			val, ok := i()
+			if !ok {
+				return s
+			} else {
+				s = s + string(val.(dafny.Char))
+			}
+		}
+	}()
+}
+func aws_cryptography_keyStore_OldEncConditionFailed_message_FromDafny(input interface{}) string {
+	return func() string {
+		var s string
+		for i := dafny.Iterate(input); ; {
+			val, ok := i()
+			if !ok {
+				return s
+			} else {
+				s = s + string(val.(dafny.Char))
+			}
+		}
+	}()
+}
+func aws_cryptography_keyStore_VersionRaceException_message_FromDafny(input interface{}) string {
 	return func() string {
 		var s string
 		for i := dafny.Iterate(input); ; {
