AwsCryptographicMaterialProviders/runtimes/java/src/main/smithy-generated/software/amazon/cryptography/keystoreadmin/model/Mutations.java
@@ -1,0 +1,144 @@
+// Copyright Amazon.com Inc. or its affiliates. All Rights Reserved.
+// SPDX-License-Identifier: Apache-2.0
+// Do not modify this file. This file is machine generated, and any changes to it will be overwritten.
+package software.amazon.cryptography.keystoreadmin.model;
+
+import java.util.Map;
+
+/**
+ *
+ * Define the Mutation in terms of the terminal, or end state,
+ * value for a particular Branch Key property.
+ * The original value will be REPLACED with this value.
+ * As of v1.8.0, a Mutation can either:
+ * - replace the KmsArn protecting the Branch Key
+ * - replace the custom encryption context
+ * - replace both the KmsArn and the custom encryption context
+ */
+public class Mutations {
+
+  /**
+   * ReEncrypt all Items of the Branch Key
+   *   to be authorized by this
+   *   AWS Key Management Service Key.
+   *   A Multi-Region or Single Region AWS KMS Key are permitted,
+   *   but not aliases!
+   */
+  private final String TerminalKmsArn;
+
+  /**
+   * ReEncrypt all Items of the Branch Key
+   *   to be authorized with this custom encryption context.
+   *   An empty Encryption Context is not allowed.
+   */
+  private final Map<String, String> TerminalEncryptionContext;
+
+  protected Mutations(BuilderImpl builder) {
+    this.TerminalKmsArn = builder.TerminalKmsArn();
+    this.TerminalEncryptionContext = builder.TerminalEncryptionContext();
+  }
+
+  /**
+   * @return ReEncrypt all Items of the Branch Key
+   *   to be authorized by this
+   *   AWS Key Management Service Key.
+   *   A Multi-Region or Single Region AWS KMS Key are permitted,
+   *   but not aliases!
+   */
+  public String TerminalKmsArn() {
+    return this.TerminalKmsArn;
+  }
+
+  /**
+   * @return ReEncrypt all Items of the Branch Key
+   *   to be authorized with this custom encryption context.
+   *   An empty Encryption Context is not allowed.
+   */
+  public Map<String, String> TerminalEncryptionContext() {
+    return this.TerminalEncryptionContext;
+  }
+
+  public Builder toBuilder() {
+    return new BuilderImpl(this);
+  }
+
+  public static Builder builder() {
+    return new BuilderImpl();
+  }
+
+  public interface Builder {
+    /**
+     * @param TerminalKmsArn ReEncrypt all Items of the Branch Key
+     *   to be authorized by this
+     *   AWS Key Management Service Key.
+     *   A Multi-Region or Single Region AWS KMS Key are permitted,
+     *   but not aliases!
+     */
+    Builder TerminalKmsArn(String TerminalKmsArn);
+
+    /**
+     * @return ReEncrypt all Items of the Branch Key
+     *   to be authorized by this
+     *   AWS Key Management Service Key.
+     *   A Multi-Region or Single Region AWS KMS Key are permitted,
+     *   but not aliases!
+     */
+    String TerminalKmsArn();
+
+    /**
+     * @param TerminalEncryptionContext ReEncrypt all Items of the Branch Key
+     *   to be authorized with this custom encryption context.
+     *   An empty Encryption Context is not allowed.
+     */
+    Builder TerminalEncryptionContext(
+      Map<String, String> TerminalEncryptionContext
+    );
+
+    /**
+     * @return ReEncrypt all Items of the Branch Key
+     *   to be authorized with this custom encryption context.
+     *   An empty Encryption Context is not allowed.
+     */
+    Map<String, String> TerminalEncryptionContext();
+
+    Mutations build();
+  }
+
+  static class BuilderImpl implements Builder {
+
+    protected String TerminalKmsArn;
+
+    protected Map<String, String> TerminalEncryptionContext;
+
+    protected BuilderImpl() {}
+
+    protected BuilderImpl(Mutations model) {
+      this.TerminalKmsArn = model.TerminalKmsArn();
+      this.TerminalEncryptionContext = model.TerminalEncryptionContext();
+    }
+
+    public Builder TerminalKmsArn(String TerminalKmsArn) {
+      this.TerminalKmsArn = TerminalKmsArn;
+      return this;
+    }
+
+    public String TerminalKmsArn() {
+      return this.TerminalKmsArn;
+    }
+
+    public Builder TerminalEncryptionContext(
+      Map<String, String> TerminalEncryptionContext
+    ) {
+      this.TerminalEncryptionContext = TerminalEncryptionContext;
+      return this;
+    }
+
+    public Map<String, String> TerminalEncryptionContext() {
+      return this.TerminalEncryptionContext;
+    }
+
+    public Mutations build() {
+      return new Mutations(this);
+    }
+  }
+}
