AwsCryptographicMaterialProviders/runtimes/net/Generated/AwsCryptographyKeyStore/WriteAtomicMutationInput.cs
@@ -1,0 +1,59 @@
+// Copyright Amazon.com Inc. or its affiliates. All Rights Reserved.
+// SPDX-License-Identifier: Apache-2.0
+// Do not modify this file. This file is machine generated, and any changes to it will be overwritten.
+using System;
+using AWS.Cryptography.KeyStore;
+namespace AWS.Cryptography.KeyStore
+{
+  public class WriteAtomicMutationInput
+  {
+    private AWS.Cryptography.KeyStore.OverWriteEncryptedHierarchicalKey _active;
+    private AWS.Cryptography.KeyStore.WriteInitializeMutationVersion _version;
+    private AWS.Cryptography.KeyStore.OverWriteEncryptedHierarchicalKey _beacon;
+    private System.Collections.Generic.List<AWS.Cryptography.KeyStore.OverWriteEncryptedHierarchicalKey> _items;
+    public AWS.Cryptography.KeyStore.OverWriteEncryptedHierarchicalKey Active
+    {
+      get { return this._active; }
+      set { this._active = value; }
+    }
+    public bool IsSetActive()
+    {
+      return this._active != null;
+    }
+    public AWS.Cryptography.KeyStore.WriteInitializeMutationVersion Version
+    {
+      get { return this._version; }
+      set { this._version = value; }
+    }
+    public bool IsSetVersion()
+    {
+      return this._version != null;
+    }
+    public AWS.Cryptography.KeyStore.OverWriteEncryptedHierarchicalKey Beacon
+    {
+      get { return this._beacon; }
+      set { this._beacon = value; }
+    }
+    public bool IsSetBeacon()
+    {
+      return this._beacon != null;
+    }
+    public System.Collections.Generic.List<AWS.Cryptography.KeyStore.OverWriteEncryptedHierarchicalKey> Items
+    {
+      get { return this._items; }
+      set { this._items = value; }
+    }
+    public bool IsSetItems()
+    {
+      return this._items != null;
+    }
+    public void Validate()
+    {
+      if (!IsSetActive()) throw new System.ArgumentException("Missing value for required property 'Active'");
+      if (!IsSetVersion()) throw new System.ArgumentException("Missing value for required property 'Version'");
+      if (!IsSetBeacon()) throw new System.ArgumentException("Missing value for required property 'Beacon'");
+      if (!IsSetItems()) throw new System.ArgumentException("Missing value for required property 'Items'");
+
+    }
+  }
+}
