AwsCryptographicMaterialProviders/dafny/AwsCryptographyKeyStoreAdmin/test/TestAdminCreateKeys.dfy
@@ -1,0 +1,137 @@
+// Copyright Amazon.com Inc. or its affiliates. All Rights Reserved.
+// SPDX-License-Identifier: Apache-2.0
+
+include "../src/Index.dfy"
+include "../../AwsCryptographyKeyStore/test/CleanupItems.dfy"
+include "../../AwsCryptographyKeyStore/test/Fixtures.dfy"
+include "../../AwsCryptographyKeyStore/Model/AwsCryptographyKeyStoreTypes.dfy"
+include "AdminFixtures.dfy"
+
+module {:options "/functionSyntax:4" } TestAdminCreateKeys {
+  import Types = AwsCryptographyKeyStoreAdminTypes
+  import KeyStoreAdmin
+  import KeyStore
+  import KeyStoreTypes = AwsCryptographyKeyStoreTypes
+  import ComAmazonawsKmsTypes
+  import KMS = Com.Amazonaws.Kms
+  import DDB = Com.Amazonaws.Dynamodb
+  import DefaultKeyStorageInterface
+  import opened Wrappers
+  import opened Fixtures
+  import UUID
+  import CleanupItems
+  import AdminFixtures
+
+  method {:test} TestCreateBranchAndBeaconKeys()
+  {
+    var ddbClient :- expect Fixtures.ProvideDDBClient();
+    var kmsClient :- expect Fixtures.ProvideKMSClient();
+    var storage :- expect Fixtures.DefaultStorage(ddbClient?:=Some(ddbClient));
+    var keyStore :- expect Fixtures.DefaultKeyStore(ddbClient?:=Some(ddbClient), kmsClient?:=Some(kmsClient));
+    var strategy :- expect AdminFixtures.DefaultKeyManagerStrategy(kmsClient?:=Some(kmsClient));
+    var underTest :- expect AdminFixtures.DefaultAdmin(ddbClient?:=Some(ddbClient));
+
+    var input := Types.CreateKeyInput(
+      Identifier := None,
+      EncryptionContext := None,
+      KmsArn := Types.KmsSymmetricKeyArn.KmsKeyArn(keyArn),
+      Strategy := Some(strategy)
+    );
+    var identifier? :- expect underTest.CreateKey(input);
+    var identifier := identifier?.Identifier;
+
+    // TODO: The rest of this is a copy/paste from KeyStore/test/TestCreateKeys.dfy
+    // We should abstract and consolidate
+    var beaconKeyResult :- expect keyStore.GetBeaconKey(
+      KeyStoreTypes.GetBeaconKeyInput(
+        branchKeyIdentifier := identifier
+      ));
+
+    var activeResult :- expect keyStore.GetActiveBranchKey(
+      KeyStoreTypes.GetActiveBranchKeyInput(
+        branchKeyIdentifier := identifier
+      ));
+
+    var branchKeyVersion :- expect UTF8.Decode(activeResult.branchKeyMaterials.branchKeyVersion);
+    var versionResult :- expect keyStore.GetBranchKeyVersion(
+      KeyStoreTypes.GetBranchKeyVersionInput(
+        branchKeyIdentifier := identifier,
+        branchKeyVersion := branchKeyVersion
+      ));
+
+    var encryptedActive :- expect storage.GetEncryptedActiveBranchKey(
+      KeyStoreTypes.GetEncryptedActiveBranchKeyInput(
+        Identifier := identifier
+      )
+    );
+
+    expect encryptedActive.Item.Type.ActiveHierarchicalSymmetricVersion?;
+    var encryptedVersion :- expect storage.GetEncryptedBranchKeyVersion(
+      KeyStoreTypes.GetEncryptedBranchKeyVersionInput(
+        Identifier := identifier,
+        Version := encryptedActive.Item.Type.ActiveHierarchicalSymmetricVersion.Version
+      )
+    );
+
+    var encryptedBeacon :- expect storage.GetEncryptedBeaconKey(
+      KeyStoreTypes.GetEncryptedBeaconKeyInput(
+        Identifier := identifier
+      )
+    );
+
+    //= aws-encryption-sdk-specification/framework/branch-key-store.md#branch-key-and-beacon-key-creation
+    //= type=test
+    //# This timestamp MUST be in ISO 8601 format in UTC, to microsecond precision (e.g. “YYYY-MM-DDTHH:mm:ss.ssssssZ“)
+    expect ISO8601?(encryptedActive.Item.CreateTime);
+    expect ISO8601?(encryptedVersion.Item.CreateTime);
+    expect ISO8601?(encryptedBeacon.Item.CreateTime);
+
+    // Since this process uses a read DDB table,
+    // the number of records will forever increase.
+    // To avoid this, remove the items.
+    CleanupItems.DeleteVersion(identifier, branchKeyVersion, ddbClient);
+    CleanupItems.DeleteActive(identifier, ddbClient);
+
+    expect beaconKeyResult.beaconKeyMaterials.beaconKey.Some?;
+    expect |beaconKeyResult.beaconKeyMaterials.beaconKey.value| == 32;
+    expect |activeResult.branchKeyMaterials.branchKey| == 32;
+    expect versionResult.branchKeyMaterials.branchKey == activeResult.branchKeyMaterials.branchKey;
+    expect versionResult.branchKeyMaterials.branchKeyIdentifier
+        == activeResult.branchKeyMaterials.branchKeyIdentifier
+        == beaconKeyResult.beaconKeyMaterials.beaconKeyIdentifier;
+    expect versionResult.branchKeyMaterials.branchKeyVersion == activeResult.branchKeyMaterials.branchKeyVersion;
+
+    //= aws-encryption-sdk-specification/framework/branch-key-store.md#createkey
+    //= type=test
+    //# If no branch key id is provided,
+    //# then this operation MUST create a [version 4 UUID](https://www.ietf.org/rfc/rfc4122.txt)
+    //# to be used as the branch key id.
+    var idByteUUID :- expect UUID.ToByteArray(activeResult.branchKeyMaterials.branchKeyIdentifier);
+    var idRoundTrip :- expect UUID.FromByteArray(idByteUUID);
+    expect idRoundTrip == activeResult.branchKeyMaterials.branchKeyIdentifier;
+
+
+    //= aws-encryption-sdk-specification/framework/branch-key-store.md#branch-key-and-beacon-key-creation
+    //= type=test
+    //# This guid MUST be [version 4 UUID](https://www.ietf.org/rfc/rfc4122.txt)
+    var versionString :- expect UTF8.Decode(activeResult.branchKeyMaterials.branchKeyVersion);
+    var versionByteUUID :- expect UUID.ToByteArray(versionString);
+    var versionRoundTrip :- expect UUID.FromByteArray(versionByteUUID);
+    expect versionRoundTrip == versionString;
+  }
+
+  predicate ISO8601?(
+    CreateTime: string
+  )
+  {
+    // “YYYY-MM-DDTHH:mm:ss.ssssssZ“
+    && |CreateTime| == 27
+    && CreateTime[4] == '-'
+    && CreateTime[7] == '-'
+    && CreateTime[10] == 'T'
+    && CreateTime[13] == ':'
+    && CreateTime[16] == ':'
+    && CreateTime[19] == '.'
+    && CreateTime[26] == 'Z'
+  }
+}
